Proving ConstFolding.v. Changed definition of Max.max_list from fold_left to fold_right.

platform/cito/Depth.v
@@ -12,7 +12,7 @@ Fixpoint depth statement :=
     | Syntax.Seq a b => max (depth a) (depth b) 
     | Syntax.If cond t f => max (edepth cond) (max (depth t) (depth f))
     | While cond body => max (edepth cond) (depth body)
-    | Syntax.Call _ f args => max (edepth f) (max_list (List.map edepth args) 0)
+    | Syntax.Call _ f args => max (edepth f) (max_list 0 (List.map edepth args))
     | Syntax.Label _ _ => 0
     | Syntax.Assign _ e => edepth e
   end.
